theories/Equ.v
@@ -265,6 +265,9 @@ Import CTree.
 Import CTreeNotations.
 Open Scope ctree.
 
+Lemma ctree_eta_ {E R} (t : ctree E R) : t ≅ go (_observe t).
+Proof. now step. Qed.
+
 Lemma ctree_eta {E R} (t : ctree E R) : t ≅ go (observe t).
 Proof.
   now step.
@@ -297,5 +300,152 @@ Lemma unfold_iter {E R I} (step : I -> ctree E (I + R)) i:
   end.
 Proof.
 	now step.
+Qed.
+
+
+Section bind.
+
+  Definition pointwise {X X' Y Y'} (SS : rel X X')
+    : rel Y Y' -> rel (X -> Y) (X' -> Y') :=
+    fun R k k' => forall x x', SS x x' -> R (k x) (k' x').
+  (* Heterogeneous [pair], todo move to library *)
+  Definition pairH {A B : Type} (x : A) (y : B) : A -> B -> Prop :=
+    fun x' y' => x = x' /\ y = y'.
+
+  Lemma leq_pairH : forall {A B : Type} (x : A) (y : B) (R : rel A B),
+      R x y <-> pairH x y <= R.
+  Proof.
+    firstorder congruence.
+  Qed.
+
+  Section Bind_ctx.
+
+    Context {E: Type -> Type} {X X' Y Y': Type}.
+
+    (* Most general contextualisation function associated to [bind]
+	   Can be read more digestly as, where R is a relation on ctrees (the prefixes of the binds) and S on the continuations:
+		 bind_ctx R S = {(bind t k, bind t' k') | R t t' /\ S k k'}
+
+		 This definition could actually be generalized,
+     the same way the Coinduction library provides generic binary contexts ([binary_ctx]).
+	   *)
+
+    (* The most general context:
+    bind_ctx R S ≜ {(bind x k, bind x' k') | R x x' /\ S k k'}
+     *)
+    Definition bind_ctx
+               (R: rel (ctree E X) (ctree E X'))
+               (S: rel (X -> ctree E Y) (X' -> ctree E Y')):
+      rel (ctree E Y) (ctree E Y') :=
+      sup_all (fun x => sup (R x) (fun x' =>
+                                  sup_all (fun k => sup (S k) (fun k' => pairH (bind x k) (bind x' k'))))).
+
+    (* Two lemmas to interact with [bind_ctx]:
+     - [leq_bind_ctx] specifies relations above the context
+     - [in_bind_ctx] specifies how to populate it *)
+    Lemma leq_bind_ctx:
+      forall R S S', bind_ctx R S <= S' <->
+                  (forall x x', R x x' -> forall k k', S k k' -> S' (bind x k) (bind x' k')).
+    Proof.
+      intros.
+      unfold bind_ctx.
+      setoid_rewrite sup_all_spec.
+      setoid_rewrite sup_spec.
+      setoid_rewrite sup_all_spec.
+      setoid_rewrite sup_spec.
+      setoid_rewrite <-leq_pairH.
+      firstorder.
+    Qed.
+
+    Lemma in_bind_ctx (R S :rel _ _) x x' y y':
+      R x x' -> S y y' -> bind_ctx R S (bind x y) (bind x' y').
+    Proof. intros. now apply ->leq_bind_ctx. Qed.
+    Global Opaque bind_ctx.
+
+  End Bind_ctx.
+
+  Section Concrete_Bind_ctx.
+
+    Context {E: Type -> Type} {X1 X2 Y1 Y2: Type}.
+
+    (* specialisation to a function acting with [equ] on the bound value, and with the argument (pointwise) on the continuation *)
+    Program Definition bind_ctx_equ SS: mon (rel (ctree E Y1) (ctree E Y2)) :=
+      {|body := fun R => @bind_ctx E X1 X2 Y1 Y2 (equ SS) (pointwise SS R) |}.
+    Next Obligation.
+      intros ??? H. apply leq_bind_ctx. intros ?? H' ?? H''.
+      apply in_bind_ctx. apply H'. intros t t' HS. apply H0, H'', HS.
+    Qed.
+
+    (* this gives a valid up-to technique *)
+    Lemma bind_ctx_equ_t (SS : rel X1 X2) (RR : rel Y1 Y2): bind_ctx_equ SS <= t_equ RR.
+    Proof.
+      apply Coinduction. intros R. apply (leq_bind_ctx _).
+      intros x x' xx' k k' kk'.
+      step in xx'.
+      cbn; unfold observe; cbn.
+      destruct xx'.
+      - cbn in *.
+        generalize (kk' _ _ REL).
+        apply (fequ RR).
+        apply id_T.
+      - constructor; intros ?. apply (fTf_Tf (fequ _)).
+        apply in_bind_ctx. apply REL.
+        red; intros. apply (b_T (fequ _)), kk'; auto.
+      - constructor. intro a. apply (fTf_Tf (fequ _)).
+        apply in_bind_ctx. apply REL.
+        red; intros. apply (b_T (fequ _)), kk'; auto.
+    Qed.
+
+  End Concrete_Bind_ctx.
+
+End bind.
+
+Lemma equ_clo_bind (E: Type -> Type) (X1 X2 Y1 Y2 : Type) :
+	forall (t1 : ctree E X1) (t2 : ctree E X2) (k1 : X1 -> ctree E Y1) (k2 : X2 -> ctree E Y2)
+    (S : rel X1 X2) (R : rel Y1 Y2) RR,
+		equ S t1 t2 ->
+    (forall x1 x2, S x1 x2 -> (t_equ R RR) (k1 x1) (k2 x2)) ->
+    t_equ R RR (bind t1 k1) (bind t2 k2)
+.
+Proof.
+  intros.
+  apply (ft_t (bind_ctx_equ_t S R)).
+  now apply in_bind_ctx.
+Qed.
+
+(* and as a consequence, one may rewrite under binds *)
+#[global] Instance bind_equ_cong :
+ forall (E : Type -> Type) (X Y : Type) (R : rel Y Y) RR,
+   Proper (equ (@eq X) ==> pointwise_relation X (t_equ R RR) ==> t_equ R RR) (@bind E X Y).
+Proof.
+  repeat red; intros; eapply equ_clo_bind; eauto.
+  intros ? ? <-; auto.
+Qed.
+
+Lemma bind_ret_l {E X Y} : forall (x : X) (k : X -> ctree E Y),
+    Ret x >>= k ≅ k x.
+Proof.
+  intros.
+  now rewrite unfold_bind.
+Qed.
+
+Lemma bind_ret_r {E X} : forall (t : ctree E X),
+    x <- t;; Ret x ≅ t.
+Proof.
+  coinduction S CIH.
+  intros t.
+  rewrite unfold_bind.
+  cbn; desobs t; constructor; auto.
+Qed.
+
+Lemma bind_bind {E X Y Z} : forall (t : ctree E X) (k : X -> ctree E Y) (l : Y -> ctree E Z),
+    (t >>= k) >>= l ≅ t >>= (fun x => k x >>= l).
+Proof.
+  coinduction S CIH; intros.
+  rewrite (ctree_eta t). cbn.
+  desobs t; cbn.
+  - reflexivity.
+  - constructor; intros. apply CIH.
+  - constructor; intros. apply CIH.
 Qed.
 
